Implement an interface for external scheduling
The compilation chain now invokes the OCaml Nlustrelib.SchedulerFun.schedule
function for each node giving the possibility to call external code to
reschedule the equations to satisfy Is_well_sch.

NLustre/nlustrelib.ml
@@ -238,3 +238,14 @@ module PrintFun (NL: SYNTAX)
       fprintf p "@]@."
   end
 
+module SchedulerFun (NL: SYNTAX) :
+  sig
+    val schedule : NL.equation list -> BinNums.positive list
+  end
+  =
+  struct
+
+    let schedule eqs = []
+
+  end
+
