NLustre/NLSchedule.v
@@ -1,0 +1,336 @@
+Require Import List.
+Import List.ListNotations.
+Open Scope list_scope.
+Require Import Coq.Sorting.Permutation.
+Require Import Coq.Sorting.Mergesort.
+
+Require Import Coq.FSets.FMapPositive.
+Require Import Velus.Common.
+Require Import Velus.Operators.
+Require Import Velus.Clocks.
+Require Import Velus.NLustre.NLSyntax.
+Require Import Velus.NLustre.Ordered.
+Require Import Velus.NLustre.Stream.
+Require Import Velus.NLustre.NLSemantics.
+
+Require Import Velus.NLustre.IsFree.
+Require Import Velus.NLustre.NLTyping.
+Require Import Velus.NLustre.Memories.
+Require Import Velus.NLustre.IsDefined.
+Require Import Velus.NLustre.NLClocking.
+
+(** * Scheduling of N-Lustre equations *)
+
+(**
+  
+  The scheduler routines are parameterized over an external scheduler
+  (EXT_NLSCHEDULER) that provides a schedule function.
+
+  The schedule function should map a list of equations to a list of priority
+  values (positive integers). If the output list has the same length as the
+  input list, the equations are sorted in ascending order of their priorities.
+
+  The idea is to allow an external scheduler to be written in OCaml. The
+  scheduler should order the equations by their dependencies. If this is
+  impossible, it should print an explanatory error message and return the
+  empty list.
+
+ *)
+
+Module Type EXT_NLSCHEDULER
+       (Import Ids   : IDS)
+       (Import Op    : OPERATORS)
+       (Import Clks  : CLOCKS   Ids)
+       (Import Syn   : NLSYNTAX Ids Op Clks).
+
+  Parameter schedule : list equation -> list positive.
+  
+End EXT_NLSCHEDULER.
+
+Module Type NLSCHEDULE
+       (Import Ids   : IDS)
+       (Import Op    : OPERATORS)
+       (Import OpAux : OPERATORS_AUX       Op)
+       (Import Clks  : CLOCKS          Ids)
+       (Import Syn   : NLSYNTAX        Ids Op       Clks)
+       (Import Ord   : ORDERED         Ids Op       Clks Syn)
+       (Import IsF   : ISFREE          Ids Op       Clks Syn)
+       (Import Str   : STREAM              Op)
+       (Import Sem   : NLSEMANTICS     Ids Op OpAux Clks Syn Str Ord)
+       (Import Typ   : NLTYPING        Ids Op       Clks Syn)
+       (Import Mem   : MEMORIES        Ids Op       Clks Syn)
+       (Import IsD   : ISDEFINED       Ids Op       Clks Syn Mem)
+       (Import Clo   : NLCLOCKING      Ids Op       Clks Syn IsF Mem IsD)
+       (Import Sch   : EXT_NLSCHEDULER Ids Op        Clks Syn).
+
+  Section OCombine.
+    Context {A B: Type}.
+
+    Fixpoint ocombine (l : list A) (l' : list B) : option (list (A * B)) :=
+      match l, l' with
+      | [], [] => Some []
+      | x::xs, y::ys =>
+        match ocombine xs ys with
+        | None => None
+        | Some rs => Some ((x, y) :: rs)
+        end
+      | _, _ => None
+      end.
+
+    Lemma ocombine_combine:
+      forall l l' ll,
+        ocombine l l' = Some ll ->
+        combine l l' = ll.
+    Proof.
+      induction l, l'; simpl;
+        try (now inversion_clear 1; auto).
+      intros ll HH.
+      destruct (ocombine l l') eqn:Hoc.
+      2:now inv HH.
+      rewrite (IHl _ _ Hoc).
+      now inv HH.
+    Qed.
+
+    Lemma ocombine_length:
+      forall l l' ll,
+        ocombine l l' = Some ll ->
+        length l = length l'.
+    Proof.
+      induction l, l'; simpl; inversion 1; auto.
+      destruct (ocombine l l') eqn:Hoc.
+      now rewrite (IHl _ _ Hoc).
+      inv H.
+    Qed.
+
+  End OCombine.
+
+  Module SchEqOrder <: Orders.TotalLeBool'.
+
+    Definition t : Type := (positive * equation)%type.
+
+    (* The arguments are inversed to put the list in the reverse order
+       expected by [Is_well_sch]. *)
+    Definition leb (s1 s2 : t) : bool := ((fst s2) <=? (fst s1))%positive.
+
+    Lemma leb_total:
+      forall s1 s2,
+        leb s1 s2 = true \/ leb s2 s1 = true.
+    Proof.
+      destruct s1 as (p1 & eq1).
+      destruct s2 as (p2 & eq2).
+      unfold leb; simpl.
+      setoid_rewrite POrderedType.Positive_as_OT.leb_compare.
+      destruct (p1 ?= p2)%positive eqn:Hp; auto.
+      apply Pos.compare_gt_iff in Hp.
+      apply Pos.compare_lt_iff in Hp.
+      rewrite Hp; auto.
+    Qed.
+
+  End SchEqOrder.
+
+  Module SchSort := Sort SchEqOrder.
+  
+  Definition schedule_eqs (eqs : list equation) : list equation :=
+    let sch := Sch.schedule eqs in
+    match ocombine sch eqs with
+    | None => eqs
+    | Some scheqs =>
+      map snd (SchSort.sort scheqs)
+    end.
+
+  Lemma map_snd_combine:
+    forall {A B} (l: list A) (l': list B),
+      length l = length l' ->
+      map snd (combine l l') = l'.
+  Proof.
+    induction l, l'; inversion 1; auto.
+    simpl. now rewrite (IHl _ H1).
+  Qed.
+  
+  Lemma schedule_eqs_permutation:
+    forall eqs,
+      Permutation (schedule_eqs eqs) eqs.
+  Proof.
+    unfold schedule_eqs.
+    intro eqs.
+    destruct (ocombine (schedule eqs) eqs) eqn:Hoc; auto.
+    rewrite <-SchSort.Permuted_sort.
+    pose proof (ocombine_length _ _ _ Hoc) as Hlen.
+    apply ocombine_combine in Hoc.
+    rewrite <-Hoc, map_snd_combine; auto.
+  Qed.
+
+  Require Import Morphisms.
+
+  Instance var_defined_Permutation_Proper:
+    Proper (@Permutation equation ==> Permutation (A:=ident)) vars_defined.
+  Proof.
+    intros eqs eqs' Hperm.
+    unfold vars_defined, concatMap.
+    induction Hperm; auto; simpl.
+    - rewrite IHHperm; auto.
+    - now rewrite <-Permutation_app_assoc,
+                  (Permutation_app_comm (var_defined y)),
+                  Permutation_app_assoc.
+    - now rewrite IHHperm1, IHHperm2.
+  Qed.
+
+  Program Definition schedule_node (n: node): node :=
+    match n with
+      mk_node name nin nout vars eqs
+              ingt0 outgt0 defd vout nodup good =>
+      mk_node name nin nout vars (schedule_eqs eqs)
+              ingt0 outgt0 _ _ nodup good
+    end.
+  Next Obligation.
+    now setoid_rewrite schedule_eqs_permutation.
+  Qed.
+  Next Obligation.
+    setoid_rewrite schedule_eqs_permutation; auto.
+  Qed.
+
+  Definition schedule (G: global) : global :=
+    map schedule_node G.
+
+  Lemma schedule_node_name:
+    forall n,
+      (schedule_node n).(n_name) = n.(n_name).
+  Proof.
+    destruct n; auto.
+  Qed.
+
+  Lemma scheduler_wc_global:
+    forall G,
+      wc_global G ->
+      wc_global (schedule G).
+  Proof.
+    intros G HG.
+    induction G as [|n G Hwc IH]; auto.
+    inv HG.
+    constructor; [|now apply Hwc].
+    inv H1.
+    destruct n.
+    constructor; auto.
+    simpl in *.
+    now rewrite schedule_eqs_permutation.
+  Qed.
+
+  Lemma schedule_map_name:
+    forall G,
+      map n_name (schedule G) = map n_name G.
+  Proof.
+    induction G as [|n G IH]; auto.
+    destruct n.
+    simpl. now rewrite IH.
+  Qed.
+
+  Lemma scheduler_find_node:
+    forall G f n,
+      find_node f G = Some n ->
+      find_node f (schedule G) = Some (schedule_node n).
+  Proof.
+    induction G as [|n' G IH]; [now inversion 1|].
+    intros f n Hfind.
+    simpl in *.
+    destruct (ident_eqb n'.(n_name) f) eqn:Heq.
+    - inv Hfind.
+      destruct n; simpl in *.
+      now rewrite Heq.
+    - destruct n'. simpl in *. rewrite Heq; auto.
+  Qed.
+
+  Lemma scheduler_find_node':
+    forall G f n,
+      find_node f (schedule G) = Some n ->
+      exists n',
+        find_node f G = Some n'
+        /\ n = schedule_node n'.
+  Proof.
+    induction G as [|n' G IH]; [now inversion 1|].
+    intros f n Hfind.
+    simpl in *.
+    destruct n'; simpl in *.
+    destruct (ident_eqb n_name0 f) eqn:Heq; eauto.
+    inv Hfind; eauto.
+  Qed.
+
+  Lemma scheduler_wt_equation:
+    forall G vars eq,
+      wt_equation G vars eq ->
+      wt_equation (schedule G) vars eq.
+  Proof.
+    induction G as [|n G IH].
+    now destruct eq; inversion_clear 1; eauto with nltyping.
+    destruct eq; inversion_clear 1; eauto with nltyping.
+    match goal with H:find_node _ _ = _ |- _ =>
+                    apply scheduler_find_node in H end.
+    destruct n0; eauto with nltyping.
+  Qed.
+
+  Lemma scheduler_wt_global:
+    forall G,
+      wt_global G ->
+      wt_global (schedule G).
+  Proof.
+    intros G HG.
+    induction G as [|n G Hwt IH]; auto.
+    inv HG. simpl.
+    apply wtg_cons; auto.
+    - unfold wt_node in *.
+      destruct n; simpl in *.
+      rewrite schedule_eqs_permutation.
+      eapply Forall_impl with (2:=H2).
+      apply scheduler_wt_equation.
+    - change (Forall (fun n'=>
+                        (fun x => n_name (schedule_node n) <> x) n'.(n_name))
+                     (schedule G)).
+      rewrite <-Forall_map.
+      rewrite schedule_map_name.
+      rewrite Forall_map.
+      destruct n; auto.
+  Qed.
+
+  Lemma scheduler_sem_node:
+    forall G f xss yss,
+      sem_node G f xss yss ->
+      sem_node (schedule G) f xss yss.
+  Proof.
+    intros G.
+    induction 1 using sem_node_mult
+    with (P := fun bk H eq Hsem =>
+                 sem_equation G bk H eq ->
+                 sem_equation (schedule G) bk H eq);
+      try (now inversion_clear 1; eauto).
+    match goal with H:find_node _ _ = _ |- _ =>
+                    apply scheduler_find_node in H end.
+    match goal with H:exists _, _ |- _ =>
+                    destruct H as (HH & Hxss & Hyss & Hsxss & Hsyss & Habs & Hsems) end.
+    econstructor; eauto.
+    exists HH; intuition.
+    rewrite schedule_eqs_permutation.
+    apply Forall_impl with (2:=Hsems).
+    intros eq Hsem.
+    destruct Hsem; auto.
+  Qed.
+  
+End NLSCHEDULE.
+
+Module NLScheduleFun
+       (Ids   : IDS)
+       (Op    : OPERATORS)
+       (OpAux : OPERATORS_AUX       Op)
+       (Clks  : CLOCKS          Ids)
+       (Syn   : NLSYNTAX        Ids Op       Clks)
+       (Ord   : ORDERED         Ids Op       Clks Syn)
+       (IsF   : ISFREE          Ids Op       Clks Syn)
+       (Str   : STREAM              Op)
+       (Sem   : NLSEMANTICS     Ids Op OpAux Clks Syn Str Ord)
+       (Typ   : NLTYPING        Ids Op       Clks Syn)
+       (Mem   : MEMORIES        Ids Op       Clks Syn)
+       (IsD   : ISDEFINED       Ids Op       Clks Syn Mem)
+       (Clo   : NLCLOCKING      Ids Op       Clks Syn IsF Mem IsD)
+       (Sch   : EXT_NLSCHEDULER Ids Op        Clks Syn)
+       <: NLSCHEDULE Ids Op OpAux Clks Syn Ord IsF Str Sem Typ Mem IsD Clo Sch.
+  Include NLSCHEDULE Ids Op OpAux Clks Syn Ord IsF Str Sem Typ Mem IsD Clo Sch.
+End NLScheduleFun.
+
